doc-src/TutorialI/Recdef/simplification.thy
@@ -7,12 +7,12 @@ Once we have succeeded in proving all termination conditions, the recursion
 equations become simplification rules, just as with
 \isacommand{primrec}. In most cases this works fine, but there is a subtle
 problem that must be mentioned: simplification may not
-terminate because of automatic splitting of @{text"if"}.
+terminate because of automatic splitting of @{text if}.
 Let us look at an example:
 *}
 
-consts gcd :: "nat\<times>nat \\<Rightarrow> nat";
-recdef gcd "measure (\\<lambda>(m,n).n)"
+consts gcd :: "nat\<times>nat \<Rightarrow> nat";
+recdef gcd "measure (\<lambda>(m,n).n)"
   "gcd (m, n) = (if n=0 then m else gcd(n, m mod n))";
 
 text{*\noindent
@@ -22,10 +22,10 @@ each recursive call. The resulting termination condition
 is provded automatically because it is already present as a lemma in the
 arithmetic library. Thus the recursion equation becomes a simplification
 rule. Of course the equation is nonterminating if we are allowed to unfold
-the recursive call inside the @{text"if"} branch, which is why programming
+the recursive call inside the @{text else} branch, which is why programming
 languages and our simplifier don't do that. Unfortunately the simplifier does
-something else which leads to the same problem: it splits @{text"if"}s if the
-condition simplifies to neither @{term"True"} nor @{term"False"}. For
+something else which leads to the same problem: it splits @{text if}s if the
+condition simplifies to neither @{term True} nor @{term False}. For
 example, simplification reduces
 @{term[display]"gcd(m,n) = k"}
 in one step to
@@ -33,23 +33,23 @@ in one step to
 where the condition cannot be reduced further, and splitting leads to
 @{term[display]"(n=0 --> m=k) & (n ~= 0 --> gcd(n, m mod n)=k)"}
 Since the recursive call @{term"gcd(n, m mod n)"} is no longer protected by
-an @{text"if"}, it is unfolded again, which leads to an infinite chain of
+an @{text if}, it is unfolded again, which leads to an infinite chain of
 simplification steps. Fortunately, this problem can be avoided in many
 different ways.
 
 The most radical solution is to disable the offending
 @{thm[source]split_if} as shown in the section on case splits in
 \S\ref{sec:Simplification}.  However, we do not recommend this because it
-means you will often have to invoke the rule explicitly when @{text"if"} is
+means you will often have to invoke the rule explicitly when @{text if} is
 involved.
 
 If possible, the definition should be given by pattern matching on the left
-rather than @{text"if"} on the right. In the case of @{term"gcd"} the
+rather than @{text if} on the right. In the case of @{term gcd} the
 following alternative definition suggests itself:
 *}
 
-consts gcd1 :: "nat\<times>nat \\<Rightarrow> nat";
-recdef gcd1 "measure (\\<lambda>(m,n).n)"
+consts gcd1 :: "nat\<times>nat \<Rightarrow> nat";
+recdef gcd1 "measure (\<lambda>(m,n).n)"
   "gcd1 (m, 0) = m"
   "gcd1 (m, n) = gcd1(n, m mod n)";
 
@@ -59,25 +59,27 @@ Note that the order of equations is important and hides the side condition
 @{prop"n ~= 0"}. Unfortunately, in general the case distinction
 may not be expressible by pattern matching.
 
-A very simple alternative is to replace @{text"if"} by @{text"case"}, which
+A very simple alternative is to replace @{text if} by @{text case}, which
 is also available for @{typ"bool"} but is not split automatically:
 *}
 
-consts gcd2 :: "nat\<times>nat \\<Rightarrow> nat";
-recdef gcd2 "measure (\\<lambda>(m,n).n)"
-  "gcd2(m,n) = (case n=0 of True \\<Rightarrow> m | False \\<Rightarrow> gcd2(n,m mod n))";
+consts gcd2 :: "nat\<times>nat \<Rightarrow> nat";
+recdef gcd2 "measure (\<lambda>(m,n).n)"
+  "gcd2(m,n) = (case n=0 of True \<Rightarrow> m | False \<Rightarrow> gcd2(n,m mod n))";
 
 text{*\noindent
 In fact, this is probably the neatest solution next to pattern matching.
 
 A final alternative is to replace the offending simplification rules by
-derived conditional ones. For @{term"gcd"} it means we have to prove
+derived conditional ones. For @{term gcd} it means we have to prove
 *}
 
 lemma [simp]: "gcd (m, 0) = m";
-by(simp);
-lemma [simp]: "n \\<noteq> 0 \\<Longrightarrow> gcd(m, n) = gcd(n, m mod n)";
-by(simp);
+apply(simp);
+done
+lemma [simp]: "n \<noteq> 0 \<Longrightarrow> gcd(m, n) = gcd(n, m mod n)";
+apply(simp);
+done
 
 text{*\noindent
 after which we can disable the original simplification rule:
