doc-src/TutorialI/Trie/Trie.thy
@@ -18,8 +18,8 @@ which is fine because products are datatypes as well.
 We define two selector functions:
 *};
 
-consts value :: "('a,'v)trie \\<Rightarrow> 'v option"
-       alist :: "('a,'v)trie \\<Rightarrow> ('a * ('a,'v)trie)list";
+consts value :: "('a,'v)trie \<Rightarrow> 'v option"
+       alist :: "('a,'v)trie \<Rightarrow> ('a * ('a,'v)trie)list";
 primrec "value(Trie ov al) = ov";
 primrec "alist(Trie ov al) = al";
 
@@ -27,7 +27,7 @@ text{*\noindent
 Association lists come with a generic lookup function:
 *};
 
-consts   assoc :: "('key * 'val)list \\<Rightarrow> 'key \\<Rightarrow> 'val option";
+consts   assoc :: "('key * 'val)list \<Rightarrow> 'key \<Rightarrow> 'val option";
 primrec "assoc [] x = None"
         "assoc (p#ps) x =
            (let (a,b) = p in if a=x then Some b else assoc ps x)";
@@ -39,20 +39,21 @@ recursion on lists is simpler than on tries, let us express this as primitive
 recursion on the search string argument:
 *};
 
-consts   lookup :: "('a,'v)trie \\<Rightarrow> 'a list \\<Rightarrow> 'v option";
+consts   lookup :: "('a,'v)trie \<Rightarrow> 'a list \<Rightarrow> 'v option";
 primrec "lookup t [] = value t"
         "lookup t (a#as) = (case assoc (alist t) a of
-                              None \\<Rightarrow> None
-                            | Some at \\<Rightarrow> lookup at as)";
+                              None \<Rightarrow> None
+                            | Some at \<Rightarrow> lookup at as)";
 
 text{*
 As a first simple property we prove that looking up a string in the empty
-trie @{term"Trie None []"} always returns @{term"None"}. The proof merely
+trie @{term"Trie None []"} always returns @{term None}. The proof merely
 distinguishes the two cases whether the search string is empty or not:
 *};
 
 lemma [simp]: "lookup (Trie None []) as = None";
-by(case_tac as, simp_all);
+apply(case_tac as, simp_all);
+done
 
 text{*
 Things begin to get interesting with the definition of an update function
@@ -60,24 +61,24 @@ that adds a new (string,value) pair to a trie, overwriting the old value
 associated with that string:
 *};
 
-consts update :: "('a,'v)trie \\<Rightarrow> 'a list \\<Rightarrow> 'v \\<Rightarrow> ('a,'v)trie";
+consts update :: "('a,'v)trie \<Rightarrow> 'a list \<Rightarrow> 'v \<Rightarrow> ('a,'v)trie";
 primrec
   "update t []     v = Trie (Some v) (alist t)"
   "update t (a#as) v =
      (let tt = (case assoc (alist t) a of
-                  None \\<Rightarrow> Trie None [] | Some at \\<Rightarrow> at)
+                  None \<Rightarrow> Trie None [] | Some at \<Rightarrow> at)
       in Trie (value t) ((a,update tt as v)#alist t))";
 
 text{*\noindent
 The base case is obvious. In the recursive case the subtrie
-@{term"tt"} associated with the first letter @{term"a"} is extracted,
+@{term tt} associated with the first letter @{term a} is extracted,
 recursively updated, and then placed in front of the association list.
-The old subtrie associated with @{term"a"} is still in the association list
-but no longer accessible via @{term"assoc"}. Clearly, there is room here for
+The old subtrie associated with @{term a} is still in the association list
+but no longer accessible via @{term assoc}. Clearly, there is room here for
 optimizations!
 
-Before we start on any proofs about @{term"update"} we tell the simplifier to
-expand all @{text"let"}s and to split all @{text"case"}-constructs over
+Before we start on any proofs about @{term update} we tell the simplifier to
+expand all @{text let}s and to split all @{text case}-constructs over
 options:
 *};
 
@@ -85,23 +86,23 @@ declare Let_def[simp] option.split[split]
 
 text{*\noindent
 The reason becomes clear when looking (probably after a failed proof
-attempt) at the body of @{term"update"}: it contains both
-@{text"let"} and a case distinction over type @{text"option"}.
+attempt) at the body of @{term update}: it contains both
+@{text let} and a case distinction over type @{text option}.
 
-Our main goal is to prove the correct interaction of @{term"update"} and
-@{term"lookup"}:
+Our main goal is to prove the correct interaction of @{term update} and
+@{term lookup}:
 *};
 
-theorem "\\<forall>t v bs. lookup (update t as v) bs =
+theorem "\<forall>t v bs. lookup (update t as v) bs =
                     (if as=bs then Some v else lookup t bs)";
 
 txt{*\noindent
-Our plan is to induct on @{term"as"}; hence the remaining variables are
+Our plan is to induct on @{term as}; hence the remaining variables are
 quantified. From the definitions it is clear that induction on either
-@{term"as"} or @{term"bs"} is required. The choice of @{term"as"} is merely
-guided by the intuition that simplification of @{term"lookup"} might be easier
-if @{term"update"} has already been simplified, which can only happen if
-@{term"as"} is instantiated.
+@{term as} or @{term bs} is required. The choice of @{term as} is merely
+guided by the intuition that simplification of @{term lookup} might be easier
+if @{term update} has already been simplified, which can only happen if
+@{term as} is instantiated.
 The start of the proof is completely conventional:
 *};
 apply(induct_tac as, auto);
@@ -113,14 +114,15 @@ Unfortunately, this time we are left with three intimidating looking subgoals:
 ~2.~\dots~{\isasymLongrightarrow}~lookup~\dots~bs~=~lookup~t~bs\isanewline
 ~3.~\dots~{\isasymLongrightarrow}~lookup~\dots~bs~=~lookup~t~bs
 \end{isabelle}
-Clearly, if we want to make headway we have to instantiate @{term"bs"} as
+Clearly, if we want to make headway we have to instantiate @{term bs} as
 well now. It turns out that instead of induction, case distinction
 suffices:
 *};
-by(case_tac[!] bs, auto);
+apply(case_tac[!] bs, auto);
+done
 
 text{*\noindent
-All methods ending in @{text"tac"} take an optional first argument that
+All methods ending in @{text tac} take an optional first argument that
 specifies the range of subgoals they are applied to, where @{text"[!]"} means
 all subgoals, i.e.\ @{text"[1-3]"} in our case. Individual subgoal numbers,
 e.g. @{text"[2]"} are also allowed.
@@ -128,8 +130,8 @@ e.g. @{text"[2]"} are also allowed.
 This proof may look surprisingly straightforward. However, note that this
 comes at a cost: the proof script is unreadable because the intermediate
 proof states are invisible, and we rely on the (possibly brittle) magic of
-@{text"auto"} (@{text"simp_all"} will not do---try it) to split the subgoals
-of the induction up in such a way that case distinction on @{term"bs"} makes
+@{text auto} (@{text simp_all} will not do---try it) to split the subgoals
+of the induction up in such a way that case distinction on @{term bs} makes
 sense and solves the proof. Part~\ref{Isar} shows you how to write readable
 and stable proofs.
 *};
