doc-src/TutorialI/Datatype/ABexpr.thy
@@ -101,7 +101,8 @@ txt{*\noindent
 The resulting 8 goals (one for each constructor) are proved in one fell swoop:
 *}
 
-by simp_all;
+apply simp_all;
+(*<*)done(*>*)
 
 text{*
 In general, given $n$ mutually recursive datatypes $\tau@1$, \dots, $\tau@n$,
