doc-src/TutorialI/Misc/arith1.thy
@@ -1,7 +1,7 @@
 (*<*)
 theory arith1 = Main:;
 (*>*)
-lemma "\\<lbrakk> \\<not> m < n; m < n+1 \\<rbrakk> \\<Longrightarrow> m = n";
+lemma "\<lbrakk> \<not> m < n; m < n+1 \<rbrakk> \<Longrightarrow> m = n";
 (**)(*<*)
 by(auto);
 end
