doc-src/TutorialI/Misc/arith2.thy
@@ -2,7 +2,8 @@
 theory arith2 = Main:;
 (*>*)
 lemma "min i (max j (k*k)) = max (min (k*k) i) (min i (j::nat))";
-by(arith);
+apply(arith);
 (**)(*<*)
+done
 end
 (*>*)
